pulse/share/steel/examples/pulse/GhostState.fst
@@ -1,0 +1,87 @@
+module GhostState
+open Pulse.Lib.Pervasives
+open Pulse.Lib.Reference
+open Pulse.Lib.SpinLock
+
+assume
+val run_stt (#a:Type) (#post:a -> vprop) (f:stt a emp post) : a
+
+type st_t =
+  | Init
+  | Next
+  | Final
+
+// assume
+// val payload_t : Type0
+
+// noeq
+// type concrete_st_t = 
+//   | CInit 
+//   | CNext : payload_t -> concrete_st_t
+//   | CState2 : payload_t -> concrete_st_t
+
+type handle_t = ref st_t
+
+let handle_has_state (h:handle_t) (s:st_t) : vprop = pts_to h #half_perm s
+
+type locked_handle_t = h:handle_t & lock (exists_ (fun s -> handle_has_state h s))
+
+// -------------------------------------------------------------------------- //
+
+[@@expect_failure]
+```pulse
+fn init' (_:unit)
+  requires emp
+  returns p:locked_handle_t
+  ensures handle_has_state p._1 Init
+{
+  let h = alloc Init;
+  share #st_t #emp_inames h #Init;
+  fold handle_has_state h Init;
+  fold handle_has_state h Init;
+  let lk = new_lock (exists_ (fun s -> handle_has_state h s));
+  let p = (| h, lk |);
+  rewrite (handle_has_state h Init)
+       as (handle_has_state p._1 Init);
+
+  // FIXME: cannot prove 
+  //   handle_has_state (Mkdtuple2?._1 x) Init 
+  // in the context
+  //   handle_has_state (Mkdtuple2?._1 p) Init
+
+  p
+}
+```
+let global_locked_handle : locked_handle_t = admit() // run_stt (init' ())
+
+#set-options "--print_implicits"
+
+[@@expect_failure]
+```pulse
+fn next' (_:unit)
+  requires handle_has_state global_locked_handle._1 Init
+  ensures handle_has_state global_locked_handle._1 Next
+{
+  acquire global_locked_handle._2;
+  with s. assert (handle_has_state global_locked_handle._1 s);
+  unfold handle_has_state global_locked_handle._1 Init;
+  unfold handle_has_state global_locked_handle._1 s;
+
+  // FIXME: cannot prove
+  //   pts_to #st_t (Mkdtuple2?._1 #handle_t #(fun h -> lock (exists_ #st_t (fun s -> handle_has_state h s))) global_locked_handle) #half_perm Init
+  // in the context
+  //   pts_to #st_t (Mkdtuple2?._1 #handle_t #(fun h -> lock (exists_ #st_t (fun s -> pts_to #st_t h #half_perm s <: Prims.Tot vprop))) global_locked_handle) #half_perm Init
+  // Issue: the unfold of
+  //   handle_has_state global_locked_handle._1 s
+  // unfolded too much, so now there is not syntactic equality 
+
+  pts_to_injective_eq #st_t #half_perm #half_perm #Init #s global_locked_handle._1;
+  rewrite (pts_to global_locked_handle._1 #half_perm s)
+       as (pts_to global_locked_handle._1 #half_perm Init);
+  gather #st_t #emp_inames global_locked_handle._1 #Init;
+  global_locked_handle._1 := Next;
+  share #st_t #emp_inames global_locked_handle._1 #Next;
+  fold handle_has_state global_locked_handle._1 Next;
+  release global_locked_handle._2;
+}
+```
